unified 1 and 2

Test/civl/large-samples/treiber-stack.bpl
@@ -9,8 +9,8 @@ type TaggedLocTreiber V = TaggedLoc (Treiber V) Unit;
 
 type X; // module type parameter
 
-var {:layer 3, 4} TreiberPool: Map (One (LocTreiber X)) (Vec X);
-var {:layer 0, 3} {:linear} TreiberPoolLow: Map (One (LocTreiber X)) (Treiber X);
+var {:layer 2, 3} TreiberPool: Map (One (LocTreiber X)) (Vec X);
+var {:layer 0, 2} {:linear} TreiberPoolLow: Map (One (LocTreiber X)) (Treiber X);
 
 /// Yield invariants
 
@@ -22,32 +22,32 @@ function {:inline} ListInDomain(t: Treiber X): bool {
   (forall x: LocNode X:: BetweenSet(t->nodes->val, t->top, None())[x] ==> Set_Contains(t->nodes->dom, One(x)))
 }
 
-yield invariant {:layer 2} TopInStack(loc_t: LocTreiber X);
+yield invariant {:layer 1} TopInStack(loc_t: LocTreiber X);
 preserves Map_Contains(TreiberPoolLow, One(loc_t));
 preserves (var loc_n := Map_At(TreiberPoolLow, One(loc_t))->top; loc_n is None || Set_Contains(Domain(TreiberPoolLow, loc_t), One(loc_n->t)));
 preserves (forall loc_n: LocNode X :: Set_Contains(Domain(TreiberPoolLow, loc_t), One(loc_n)) ==>
               (var loc_n' := Map_At(Map_At(TreiberPoolLow, One(loc_t))->nodes, One(loc_n))->next;
                 loc_n' is None || Set_Contains(Domain(TreiberPoolLow, loc_t), One(loc_n'->t))));
 
-yield invariant {:layer 2} LocInStackOrNone(loc_t: LocTreiber X, loc_n: Option (LocNode X));
+yield invariant {:layer 1} LocInStackOrNone(loc_t: LocTreiber X, loc_n: Option (LocNode X));
 preserves Map_Contains(TreiberPoolLow, One(loc_t));
 preserves loc_n is None || Set_Contains(Domain(TreiberPoolLow, loc_t), One(loc_n->t));
 
-yield invariant {:layer 2} LocInStack(loc_t: LocTreiber X, loc_n: LocNode X);
+yield invariant {:layer 1} LocInStack(loc_t: LocTreiber X, loc_n: LocNode X);
 preserves Map_Contains(TreiberPoolLow, One(loc_t));
 preserves Set_Contains(Domain(TreiberPoolLow, loc_t), One(loc_n));
 
-yield invariant {:layer 3} ReachInStack(loc_t: LocTreiber X);
+yield invariant {:layer 2} ReachInStack(loc_t: LocTreiber X);
 preserves Map_Contains(TreiberPoolLow, One(loc_t));
 preserves (var t := Map_At(TreiberPoolLow, One(loc_t)); Between(t->nodes->val, t->top, t->top, None()));
 preserves (var t := Map_At(TreiberPoolLow, One(loc_t)); ListInDomain(t));
 preserves (var loc_n := Map_At(TreiberPoolLow, One(loc_t))->top; loc_n is None || Set_Contains(Domain(TreiberPoolLow, loc_t), One(loc_n->t)));
 preserves Map_At(TreiberPool, One(loc_t)) == Abs(Map_At(TreiberPoolLow, One(loc_t)));
 
-yield invariant {:layer 3} StackDom();
+yield invariant {:layer 2} StackDom();
 preserves TreiberPool->dom == TreiberPoolLow->dom;
 
-yield invariant {:layer 3} PushLocInStack(loc_t: LocTreiber X, node: Node X, new_loc_n: LocNode X, {:linear} tagged_loc: One (TaggedLocNode X));
+yield invariant {:layer 2} PushLocInStack(loc_t: LocTreiber X, node: Node X, new_loc_n: LocNode X, {:linear} tagged_loc: One (TaggedLocNode X));
 preserves Map_Contains(TreiberPoolLow, One(loc_t));
 preserves Set_Contains(Domain(TreiberPoolLow, loc_t), One(new_loc_n));
 preserves tagged_loc->val == TaggedLoc(new_loc_n, Unit());
@@ -55,7 +55,7 @@ preserves (var t := Map_At(TreiberPoolLow, One(loc_t)); Map_At(t->nodes, One(new
 
 /// Layered implementation
 
-atomic action {:layer 4} AtomicAlloc() returns ({:linear} tagged_loc: One (TaggedLocTreiber X))
+atomic action {:layer 3} AtomicAlloc() returns ({:linear} tagged_loc: One (TaggedLocTreiber X))
 {
   var one_loc_t: One (LocTreiber X);
   var tagged_locs: Set (One (TaggedLocTreiber X));
@@ -66,7 +66,7 @@ atomic action {:layer 4} AtomicAlloc() returns ({:linear} tagged_loc: One (Tagge
   assume !Map_Contains(TreiberPool, one_loc_t);
   TreiberPool := Map_Update(TreiberPool, one_loc_t, Vec_Empty());
 }
-yield procedure {:layer 3} Alloc() returns ({:linear} tagged_loc: One (TaggedLocTreiber X))
+yield procedure {:layer 2} Alloc() returns ({:linear} tagged_loc: One (TaggedLocTreiber X))
 refines AtomicAlloc;
 ensures call TopInStack(tagged_loc->val->loc);
 ensures call ReachInStack(tagged_loc->val->loc);
@@ -85,11 +85,11 @@ preserves call StackDom();
   tagged_loc := One(TaggedLoc(one_loc_t->val, Unit()));
   call One_Get(tagged_locs, tagged_loc);
   call AllocTreiber#0(one_loc_t, treiber);
-  call {:layer 3} TreiberPool := Copy(Map_Update(TreiberPool, one_loc_t, Vec_Empty()));
-  call {:layer 3} AbsLemma(treiber);
+  call {:layer 2} TreiberPool := Copy(Map_Update(TreiberPool, one_loc_t, Vec_Empty()));
+  call {:layer 2} AbsLemma(treiber);
 }
 
-atomic action {:layer 4} AtomicPush(loc_t: LocTreiber X, x: X) returns (success: bool)
+atomic action {:layer 3} AtomicPush(loc_t: LocTreiber X, x: X) returns (success: bool)
 {
   if (*) {
     TreiberPool := Map_Update(TreiberPool, One(loc_t), Vec_Append(Map_At(TreiberPool, One(loc_t)), x));
@@ -98,7 +98,7 @@ atomic action {:layer 4} AtomicPush(loc_t: LocTreiber X, x: X) returns (success:
     success := false;
   }
 }
-yield procedure {:layer 3} {:vcs_split_on_every_assert} Push(loc_t: LocTreiber X, x: X) returns (success: bool)
+yield procedure {:layer 2} {:vcs_split_on_every_assert} Push(loc_t: LocTreiber X, x: X) returns (success: bool)
 refines AtomicPush;
 preserves call TopInStack(loc_t);
 preserves call ReachInStack(loc_t);
@@ -107,21 +107,21 @@ preserves call StackDom();
   var loc_n: Option (LocNode X);
   var new_loc_n: LocNode X;
   var tagged_loc: One (TaggedLocNode X);
-  var {:layer 3} old_treiber: Treiber X;
+  var {:layer 2} old_treiber: Treiber X;
 
-  call {:layer 3} old_treiber := Copy(TreiberPoolLow->val[One(loc_t)]);
+  call {:layer 2} old_treiber := Copy(TreiberPoolLow->val[One(loc_t)]);
   call loc_n, new_loc_n, tagged_loc := CreateNewTopOfStack(loc_t, x);
-  call {:layer 3} FrameLemma(old_treiber, TreiberPoolLow->val[One(loc_t)]);
+  call {:layer 2} FrameLemma(old_treiber, TreiberPoolLow->val[One(loc_t)]);
   call ReachInStack(loc_t) | StackDom() | PushLocInStack(loc_t, Node(loc_n, x), new_loc_n, tagged_loc);
   call success := WriteTopOfStack#0(loc_t, loc_n, Some(new_loc_n));
   if (success) {
-    call {:layer 3} TreiberPool := Copy(Map_Update(TreiberPool, One(loc_t), Vec_Append(Map_At(TreiberPool, One(loc_t)), x)));
-    assert {:layer 3} TreiberPoolLow->val[One(loc_t)]->top != None();
-    call {:layer 3} AbsLemma(TreiberPoolLow->val[One(loc_t)]);
+    call {:layer 2} TreiberPool := Copy(Map_Update(TreiberPool, One(loc_t), Vec_Append(Map_At(TreiberPool, One(loc_t)), x)));
+    assert {:layer 2} TreiberPoolLow->val[One(loc_t)]->top != None();
+    call {:layer 2} AbsLemma(TreiberPoolLow->val[One(loc_t)]);
   }
 }
 
-atomic action {:layer 4} AtomicPop(loc_t: LocTreiber X) returns (success: bool, x_opt: Option X)
+atomic action {:layer 3} AtomicPop(loc_t: LocTreiber X) returns (success: bool, x_opt: Option X)
 {
   var stack: Vec X;
 
@@ -139,21 +139,21 @@ atomic action {:layer 4} AtomicPop(loc_t: LocTreiber X) returns (success: bool, 
     x_opt := None();
   }
 }
-yield procedure {:layer 3} Pop(loc_t: LocTreiber X) returns (success: bool, x_opt: Option X)
+yield procedure {:layer 2} Pop(loc_t: LocTreiber X) returns (success: bool, x_opt: Option X)
 refines AtomicPop;
 preserves call TopInStack(loc_t);
 preserves call ReachInStack(loc_t);
 preserves call StackDom();
 {
-  call {:layer 3} AbsLemma(TreiberPoolLow->val[One(loc_t)]);
+  call {:layer 2} AbsLemma(TreiberPoolLow->val[One(loc_t)]);
   call success, x_opt := PopIntermediate(loc_t);
   if (x_opt is Some) {
-    assert {:layer 3} Vec_Len(Map_At(TreiberPool, One(loc_t))) > 0;
-    call {:layer 3} TreiberPool := Copy(Map_Update(TreiberPool, One(loc_t), Vec_Remove(Map_At(TreiberPool, One(loc_t)))));
+    assert {:layer 2} Vec_Len(Map_At(TreiberPool, One(loc_t))) > 0;
+    call {:layer 2} TreiberPool := Copy(Map_Update(TreiberPool, One(loc_t), Vec_Remove(Map_At(TreiberPool, One(loc_t)))));
   }
 }
 
-atomic action {:layer 3} AtomicCreateNewTopOfStack(loc_t: LocTreiber X, x: X)
+atomic action {:layer 2} AtomicCreateNewTopOfStack(loc_t: LocTreiber X, x: X)
   returns (loc_n: Option (LocNode X), new_loc_n: LocNode X, {:linear} tagged_loc: One (TaggedLocNode X))
 asserts Map_Contains(TreiberPoolLow, One(loc_t));
 {
@@ -176,10 +176,10 @@ asserts Map_Contains(TreiberPoolLow, One(loc_t));
   treiber := Treiber(top, stack);
   call Map_Put(TreiberPoolLow, one_loc_t, treiber);
 }
-yield procedure {:layer 2} CreateNewTopOfStack(loc_t: LocTreiber X, x: X)
+yield procedure {:layer 1} CreateNewTopOfStack(loc_t: LocTreiber X, x: X)
   returns (loc_n: Option (LocNode X), new_loc_n: LocNode X, {:linear} tagged_loc: One (TaggedLocNode X))
 preserves call TopInStack(loc_t);
-ensures call LocInStackOrNone(loc_t, Some(new_loc_n));
+ensures call LocInStack(loc_t, new_loc_n);
 refines AtomicCreateNewTopOfStack;
 {
   var one_loc_n: One (LocNode X);
@@ -194,7 +194,7 @@ refines AtomicCreateNewTopOfStack;
   call AllocNode#0(loc_t, one_loc_n, Node(loc_n, x));
 }
 
-atomic action {:layer 3} AtomicPopIntermediate(loc_t: LocTreiber X) returns (success: bool, x_opt: Option X)
+atomic action {:layer 2} AtomicPopIntermediate(loc_t: LocTreiber X) returns (success: bool, x_opt: Option X)
 {
   var one_loc_t: One (LocTreiber X);
   var loc_n: Option (LocNode X);
@@ -224,7 +224,7 @@ atomic action {:layer 3} AtomicPopIntermediate(loc_t: LocTreiber X) returns (suc
     success := false;
   }
 }
-yield procedure {:layer 2} PopIntermediate(loc_t: LocTreiber X) returns (success: bool, x_opt: Option X)
+yield procedure {:layer 1} PopIntermediate(loc_t: LocTreiber X) returns (success: bool, x_opt: Option X)
 refines AtomicPopIntermediate;
 preserves call TopInStack(loc_t);
 {
@@ -252,7 +252,7 @@ preserves call TopInStack(loc_t);
 /// Primitives
 
 yield procedure {:layer 0} LoadNode#0(loc_t: LocTreiber X, loc_n: LocNode X) returns (node: Node X);
-refines right action {:layer 1,2} _
+refines right action {:layer 1} _
 {
   assert Map_Contains(TreiberPoolLow, One(loc_t));
   assert Map_Contains(Map_At(TreiberPoolLow, One(loc_t))->nodes, One(loc_n));
@@ -260,7 +260,7 @@ refines right action {:layer 1,2} _
 }
 
 yield procedure {:layer 0} ReadTopOfStack#0(loc_t: LocTreiber X) returns (loc_n: Option (LocNode X));
-refines atomic action {:layer 1,2} _
+refines atomic action {:layer 1} _
 {
   assert Map_Contains(TreiberPoolLow, One(loc_t));
   loc_n := TreiberPoolLow->val[One(loc_t)]->top;
@@ -268,7 +268,7 @@ refines atomic action {:layer 1,2} _
 
 yield procedure {:layer 0} WriteTopOfStack#0(
   loc_t: LocTreiber X, old_loc_n: Option (LocNode X), new_loc_n: Option (LocNode X)) returns (success: bool);
-refines atomic action {:layer 1,3} _
+refines atomic action {:layer 1,2} _
 {
   assert Map_Contains(TreiberPoolLow, One(loc_t));
   if (old_loc_n == TreiberPoolLow->val[One(loc_t)]->top) {
@@ -280,7 +280,7 @@ refines atomic action {:layer 1,3} _
 }
 
 yield procedure {:layer 0} AllocNode#0(loc_t: LocTreiber X, {:linear_in} one_loc_n: One (LocNode X), node: Node X);
-refines atomic action {:layer 1,2} _
+refines atomic action {:layer 1} _
 {
   var one_loc_t: One (LocTreiber X);
   var treiber: Treiber X;
@@ -292,7 +292,7 @@ refines atomic action {:layer 1,2} _
 }
 
 yield procedure {:layer 0} AllocTreiber#0({:linear_in} one_loc_t: One (LocTreiber X), {:linear_in} treiber: Treiber X);
-refines atomic action {:layer 1,3} _
+refines atomic action {:layer 1,2} _
 {
   call Map_Put(TreiberPoolLow, one_loc_t, treiber);
 }
